Work (in progress) on cleaning up basis library
Move Commandline module to the new naming scheme.

Create some convenience libraries (cfLib, basis) for simplifying opens.

Move some things to misc.
Add some more to option_monadsyntax.

misc/preamble.sml
@@ -27,6 +27,7 @@ val has_pair_type = can dest_prod o type_of
 
 val option_bind_tm = prim_mk_const{Thy="option",Name="OPTION_BIND"};
 val option_ignore_bind_tm = prim_mk_const{Thy="option",Name="OPTION_IGNORE_BIND"};
+val option_guard_tm = prim_mk_const{Thy="option",Name="OPTION_GUARD"};
 
 structure option_monadsyntax = struct
 fun temp_add_option_monadsyntax() =
@@ -36,6 +37,7 @@ fun temp_add_option_monadsyntax() =
     val _ = temp_inferior_overload_on ("fail", optionSyntax.none_tm)
     val _ = temp_overload_on ("monad_bind", option_bind_tm)
     val _ = temp_overload_on ("monad_unitbind", option_ignore_bind_tm)
+    val _ = temp_overload_on ("assert", option_guard_tm)
   in () end
 
 fun add_option_monadsyntax() =
@@ -45,6 +47,7 @@ fun add_option_monadsyntax() =
     val _ = inferior_overload_on ("fail", optionSyntax.none_tm)
     val _ = overload_on ("monad_bind", option_bind_tm)
     val _ = overload_on ("monad_unitbind", option_ignore_bind_tm)
+    val _ = overload_on ("assert", option_guard_tm)
   in () end
 end
 
