basis/mlbasicsProgScript.sml
@@ -1,6 +1,7 @@
 open preamble
-     ml_translatorTheory ml_translatorLib semanticPrimitivesTheory basisFunctionsLib
-     cfHeapsTheory cfTheory cfTacticsBaseLib cfTacticsLib ml_progLib mlstringProgTheory
+     semanticPrimitivesTheory ml_translatorTheory
+     ml_translatorLib ml_progLib cfLib basisFunctionsLib
+     mlstringProgTheory
 
 val _ = new_theory "mlbasicsProg"
 
